FindDeallocable

disk-betree/IndirectionTableImpl.i.dfy
@@ -287,83 +287,50 @@ module IndirectionTableImpl {
     
     ///// Dealloc stuff
 
-    /*
-    predicate deallocable(self: IndirectionTable, ref: BT.G.Reference)
+    method Deallocable(ref: BT.G.Reference) returns (result: bool)
+    requires Inv()
+    ensures result == IndirectionTableModel.deallocable(I(), ref)
     {
-      && ref in I(self).graph
-      && ref != BT.G.Root()
-      && (forall r | r in I(self).graph :: ref !in I(self).graph[r])
-    }
-
-    function FindDeallocableIterate(self: IndirectionTable, ephemeralRefs: seq<BT.G.Reference>, i: uint64)
-    : (ref: Option<BT.G.Reference>)
-    requires 0 <= i as int <= |ephemeralRefs|
-    requires |ephemeralRefs| < 0x1_0000_0000_0000_0000;
-    decreases 0x1_0000_0000_0000_0000 - i as int
-    {
-      if i == |ephemeralRefs| as uint64 then (
-        None
-      ) else (
-        var ref := ephemeralRefs[i];
-        var isDeallocable := deallocable(self, ref);
-        if isDeallocable then (
-          Some(ref)
-        ) else (
-          FindDeallocableIterate(self, ephemeralRefs, i + 1)
-        )
-      )
-    }
-
-    function {:opaque} FindDeallocable(self: IndirectionTable)
-    : (ref: Option<BT.G.Reference>)
-    requires Inv(self)
-    {
-      // TODO once we have an lba freelist, rewrite this to avoid extracting a `map` from `s.ephemeralIndirectionTable`
-      var ephemeralRefs := setToSeq(self.t.contents.Keys);
-
-      assume |ephemeralRefs| < 0x1_0000_0000_0000_0000;
-
-      FindDeallocableIterate(self, ephemeralRefs, 0)
-    }
-
-    lemma FindDeallocableIterateCorrect(self: IndirectionTable, ephemeralRefs: seq<BT.G.Reference>, i: uint64)
-    requires Inv(self)
-    requires 0 <= i as int <= |ephemeralRefs|
-    requires |ephemeralRefs| < 0x1_0000_0000_0000_0000;
-    requires ephemeralRefs == setToSeq(self.t.contents.Keys)
-    requires forall k : nat | k < i as nat :: (
-          && ephemeralRefs[k] in I(self).graph
-          && !deallocable(self, ephemeralRefs[k]))
-    ensures var ref := FindDeallocableIterate(self, ephemeralRefs, i);
-        && (ref.Some? ==> ref.value in I(self).graph)
-        && (ref.Some? ==> deallocable(self, ref.value))
-        && (ref.None? ==> forall r | r in I(self).graph :: !deallocable(self, r))
-    decreases 0x1_0000_0000_0000_0000 - i as int
-    {
-      if i == |ephemeralRefs| as uint64 {
-        assert forall r | r in I(self).graph :: !deallocable(self, r);
-      } else {
-        var ref := ephemeralRefs[i];
-        var isDeallocable := deallocable(self, ref);
-        if isDeallocable {
-        } else {
-          FindDeallocableIterateCorrect(self, ephemeralRefs, i + 1);
-        }
+      if ref == BT.G.Root() {
+        return false;
       }
+      var lbaGraph := this.t.Get(ref);
+      if !lbaGraph.Some? {
+        return false;
+      }
+      assert ref in I().graph;
+      var table := t.ToMap();
+      var graph := map k | k in table :: table[k].succs;
+      assert graph == I().graph;
+      result := forall r | r in graph :: ref !in graph[r];
     }
 
-    lemma FindDeallocableCorrect(self: IndirectionTable)
-    requires Inv(self)
-    ensures var ref := FindDeallocable(self);
-        && (ref.Some? ==> ref.value in I(self).graph)
-        && (ref.Some? ==> deallocable(self, ref.value))
-        && (ref.None? ==> forall r | r in I(self).graph :: !deallocable(self, r))
+    method FindDeallocable() returns (ref: Option<BT.G.Reference>)
+    requires Inv()
+    ensures ref == IndirectionTableModel.FindDeallocable(I())
     {
-      reveal_FindDeallocable();
-      var ephemeralRefs := setToSeq(self.t.contents.Keys);
+      IndirectionTableModel.reveal_FindDeallocable();
+
+      // TODO once we have an lba freelist, rewrite this to avoid extracting a `map` from `s.ephemeralIndirectionTable`
+      var ephemeralTable := t.ToMap();
+      var ephemeralRefs := SetToSeq(ephemeralTable.Keys);
+
       assume |ephemeralRefs| < 0x1_0000_0000_0000_0000;
-      FindDeallocableIterateCorrect(self, ephemeralRefs, 0);
+
+      var i: uint64 := 0;
+      while i < |ephemeralRefs| as uint64
+      invariant 0 <= i as int <= |ephemeralRefs|
+      invariant IndirectionTableModel.FindDeallocableIterate(I(), ephemeralRefs, i)
+             == IndirectionTableModel.FindDeallocable(I())
+      {
+        var ref := ephemeralRefs[i];
+        var isDeallocable := this.Deallocable(ref);
+        if isDeallocable {
+          return Some(ref);
+        }
+        i := i + 1;
+      }
+      return None;
     }
-    */
   }
 }
