disk-betree/ImplDealloc.i.dfy
@@ -18,30 +18,6 @@ module ImplDealloc {
 
   import opened NativeTypes
 
-  method Deallocable(s: ImplVariables, ref: BT.G.Reference) returns (result: bool)
-  requires s.W()
-  requires s.ready ==> s.ephemeralIndirectionTable.Inv()
-  ensures result == ImplModelDealloc.deallocable(s.I(), ref)
-  {
-    if ref == BT.G.Root() {
-      return false;
-    }
-    assert ref != BT.G.Root();
-    if !s.ready {
-      return false;
-    }
-    assert s.ready;
-    var lbaGraph := s.ephemeralIndirectionTable.Get(ref);
-    if !lbaGraph.Some? {
-      return false;
-    }
-    assert ref in IM.IIndirectionTable(IIndirectionTable(s.ephemeralIndirectionTable)).graph;
-    var table := s.ephemeralIndirectionTable.ToMap();
-    var graph := map k | k in table :: table[k].1;
-    assert graph == IM.IIndirectionTable(IIndirectionTable(s.ephemeralIndirectionTable)).graph;
-    result := forall r | r in graph :: ref !in graph[r];
-  }
-
   method Dealloc(k: ImplConstants, s: ImplVariables, io: DiskIOHandler, ref: BT.G.Reference)
   requires Inv(k, s)
   requires io.initialized()
@@ -104,27 +80,5 @@ module ImplDealloc {
   requires s.ready
   ensures ref == ImplModelDealloc.FindDeallocable(s.I())
   {
-    ImplModelDealloc.reveal_FindDeallocable();
-
-    // TODO once we have an lba freelist, rewrite this to avoid extracting a `map` from `s.ephemeralIndirectionTable`
-    var ephemeralTable := s.ephemeralIndirectionTable.ToMap();
-    var ephemeralRefs := SetToSeq(ephemeralTable.Keys);
-
-    assume |ephemeralRefs| < 0x1_0000_0000_0000_0000;
-
-    var i: uint64 := 0;
-    while i < |ephemeralRefs| as uint64
-    invariant 0 <= i as int <= |ephemeralRefs|
-    invariant ImplModelDealloc.FindDeallocableIterate(s.I(), ephemeralRefs, i)
-           == ImplModelDealloc.FindDeallocable(s.I())
-    {
-      var ref := ephemeralRefs[i];
-      var isDeallocable := Deallocable(s, ref);
-      if isDeallocable {
-        return Some(ref);
-      }
-      i := i + 1;
-    }
-    return None;
   }
 }
